theories/ExprI.v
@@ -332,111 +332,6 @@ Section Expr.
   Qed.
 
 (*
-  Theorem exprD'_strengthenU_multi (EOk : ExprOk Expr_expr)
-  : forall tus tvs e  t' tus' val,
-      (forall u, u < length tus' ->
-                 mentionsU (length tus + u) e = false) ->
-      exprD' (tus ++ tus') tvs e t' = Some val ->
-      exists val',
-        exprD' tus tvs e t' = Some val' /\
-        forall us vs us',
-          val (hlist_app us us') vs = val' us vs.
-  Proof.
-    intros tus tvs e t'.
-    refine (@list_rev_ind _ _ _ _).
-    { simpl. intros.
-      rewrite exprD'_conv with (pfu := app_nil_r_trans tus) (pfv := eq_refl).
-      rewrite H0. autorewrite with eq_rw.
-      eexists; split; eauto.
-      intros. rewrite (hlist_eta us').
-      rewrite hlist_app_nil_r. reflexivity. }
-    { intros.
-      rewrite exprD'_conv with (pfu := app_ass_trans tus ls (l :: nil)) (pfv := eq_refl) in H1.
-      autorewrite with eq_rw in H1.
-      forward.
-      eapply exprD'_strengthenU_single in H1.
-      + forward_reason.
-        eapply H in H1.
-        - forward_reason.
-          eexists; split; eauto.
-          intros. inv_all; subst.
-          clear - H3 H4.
-          specialize (H4 us vs (fst (hlist_split _ _ us'))).
-          specialize (H3 (hlist_app us (fst (hlist_split _ _ us')))
-                         vs (hlist_hd (snd (hlist_split _ _ us')))).
-          rewrite <- H4; clear H4.
-          rewrite <- H3; clear H3.
-          repeat rewrite eq_Arr_eq. repeat rewrite eq_Const_eq.
-          f_equal.
-          rewrite hlist_app_assoc.
-          autorewrite with eq_rw.
-          f_equal.
-          eapply match_eq_match_eq.
-          f_equal.
-          etransitivity. symmetry. eapply (hlist_app_hlist_split _ _ us').
-          f_equal.
-          rewrite (hlist_eta (snd (hlist_split _ _ _))).
-          simpl. f_equal.
-          rewrite (hlist_eta (hlist_tl _)). reflexivity.
-        - intros.
-          eapply H0. rewrite app_length. simpl. omega.
-      + rewrite app_length.
-        apply H0. rewrite app_length. simpl. omega. }
-  Qed.
-
-
-  Theorem exprD'_strengthenV_multi (EOk : ExprOk Expr_expr)
-  : forall tus tvs e  t' tvs' val,
-      (forall v, v < length tvs' ->
-                 mentionsV (length tvs + v) e = false) ->
-      exprD' tus (tvs ++ tvs') e t' = Some val ->
-      exists val',
-        exprD' tus tvs e t' = Some val' /\
-        forall us vs vs',
-          val us (hlist_app vs vs') = val' us vs.
-  Proof.
-    intros tus tvs e t'.
-    refine (@list_rev_ind _ _ _ _).
-    { simpl. intros.
-      rewrite exprD'_conv with (pfv := app_nil_r_trans tvs) (pfu := eq_refl).
-      rewrite H0. autorewrite with eq_rw.
-      eexists; split; eauto.
-      intros. rewrite (hlist_eta vs').
-      rewrite hlist_app_nil_r.
-      reflexivity. }
-    { intros.
-      rewrite exprD'_conv with (pfv := app_ass_trans tvs ls (l :: nil)) (pfu := eq_refl) in H1.
-      autorewrite with eq_rw in H1.
-      forward.
-      eapply exprD'_strengthenV_single in H1.
-      + forward_reason.
-        eapply H in H1.
-        - forward_reason.
-          eexists; split; eauto.
-          intros. inv_all; subst.
-          clear - H3 H4.
-          specialize (H4 us vs (fst (hlist_split _ _ vs'))).
-          specialize (H3 us (hlist_app vs (fst (hlist_split _ _ vs')))
-                         (hlist_hd (snd (hlist_split _ _ vs')))).
-          rewrite <- H4; clear H4.
-          rewrite <- H3; clear H3.
-          autorewrite with eq_rw.
-          f_equal.
-          rewrite hlist_app_assoc.
-          apply match_eq_match_eq.
-          f_equal.
-          etransitivity.
-          symmetry.
-          eapply (hlist_app_hlist_split _ _ vs').
-          f_equal.
-          rewrite (hlist_eta (snd (hlist_split _ _ _))).
-          simpl. f_equal.
-          rewrite (hlist_eta (hlist_tl _)). reflexivity.
-        - intros.
-          eapply H0. rewrite app_length. simpl. omega.
-      + rewrite app_length.
-        apply H0. rewrite app_length. simpl. omega. }
-  Qed.
 *)
 
 End Expr.
@@ -445,10 +340,6 @@ Arguments Safe_expr {_ _ _ Expr} _ _ _ _ : rename.
 Arguments exprD' {_ _ _ Expr} _ _ _ _ : rename.
 Arguments exprD {_ _ _ Expr} _ _ _ _ : rename.
 Arguments exprT {_ RType} _ _ _ : rename.
-(*
-Arguments mentionsU {_ RType _ Expr} _ _ : rename.
-Arguments mentionsV {_ RType _ Expr} _ _ : rename.
-*)
 Arguments exprT_Inj {_ _} _ _ {_} _ _ _ : rename.
 Arguments exprT_UseU {_ _} tus tvs n : rename.
 Arguments exprT_UseV {_ _} tus tvs n : rename.
